Checkpoint

formal/pi/pi.c
@@ -1,0 +1,4 @@
+double pi() {
+  double c = -3.1415926535897932e+03;
+  return c;
+}
