formal/task01/build1.c
@@ -11,16 +11,17 @@ int main(void) {
     State state = {.item = {0.0, 0.0, 0.0}};
 
     // Run the simulation, saving the list of states.
-    StateList *states = run_sim(state, tstop, dt);
+    StateList *states = run_sim(&state, tstop, dt);
 
     // Print results to file and console.
     char filename[50] = "output.dat";
     FILE *f = fopen(filename, "w");
     if (!f) exit(2);
     for (StateList* cell = states; cell; cell = cell->next) {
-        double time = cell->data.item[TimeItem];
-        double x = cell->data.item[PositionItem];
-        double xd = cell->data.item[VelocityItem];
+        State* data = cell->data;
+        double time = data->item[TimeItem];
+        double x = data->item[PositionItem];
+        double xd = data->item[VelocityItem];
         printf("%3.15e\t%3.15e\t%3.15e\t\n", time, x, xd);
         fprintf(f, "%3.15e\t%3.15e\t%3.15e\t\n", time, x, xd);
     }
