formal/task01/diffeq.c
@@ -1,24 +1,23 @@
 #include "state.h"
 
 // Return first derivative of state components
-State diffeq(State state) {
+void diffeq(State* state, State* derivatives_out) {
   double damping_coefficient =  8.88;
   double gravity             =  9.88;
   double mass                =  1.00;
   double spring_coefficient  = 39.47;
 
   // Unpack state into locals.
-  double time = state.item[TimeItem];
-  double x = state.item[PositionItem];
-  double xd = state.item[VelocityItem];
-  
+  double time = state->item[TimeItem];
+  double x = state->item[PositionItem];
+  double xd = state->item[VelocityItem];
+
   State result;
   // dt/dt = 1.0
-  result.item[TimeItem] = 1.0;
+  derivatives_out->item[TimeItem] = 1.0;
   // dx/dt = velocity
-  result.item[PositionItem] = xd;
+  derivatives_out->item[PositionItem] = xd;
   // acceleration = dv/dt
-  result.item[VelocityItem] = -(spring_coefficient*x + damping_coefficient*xd)/mass - gravity;
-  return result;
+  derivatives_out->item[VelocityItem] = -(spring_coefficient*x + damping_coefficient*xd)/mass - gravity;
 }
 
