formal/task01/run_sim.c
@@ -3,26 +3,27 @@
 #include <math.h>
 #include "state.h"
 
-StateList* run_sim(State state, double tstop, double dt) {
+StateList* run_sim(State* state, double tstop, double dt) {
 
     // Get list to accumulate results.
     StateList* states = NULL;
 
     // Main simulation loop
     int i = 0;
-    while (state.item[TimeItem] <= tstop) {
+    while (state->item[TimeItem] <= tstop) {
         // Record state.
         states = state_list_cons(states, state);
 
         // Calculate derivative from current state.
-        State derivatives = diffeq(state);
+        State derivatives;
+        diffeq(state, &derivatives);
 
         // Advance state one time step
-        one_step(&state, &derivatives, dt);
+        one_step(state, &derivatives, dt);
 
         // Kludge to get time showing up nicely.
         i++;
-        state.item[TimeItem] = round(i * dt * 1.0e6) / 1.0e6;
+        state->item[TimeItem] = round(i * dt * 1.0e6) / 1.0e6;
     }
     states = reverse_state_list(states);
     return states;
