formal/task01/state.h
@@ -16,16 +16,18 @@ typedef struct s_state {
 } State;
 
 typedef struct s_state_list {
-  State data;
+  State* data;
   struct s_state_list* next;
 } StateList;
 
-StateList* new_state_list(State data, StateList* next);
-StateList* state_list_cons(StateList* list, State item);
+void copy_state(State* dest, State* src);
+State* clone_state(State* data);
+StateList* new_state_list(State* data, StateList* next);
+StateList* state_list_cons(StateList* list, State* item);
 StateList* reverse_state_list(StateList* list);
   
 // Return first derivative of state components
-State diffeq(State state);
+void diffeq(State* state_in, State* derivatives_out);
 
 // Update state given derivatives and time delta.
 void one_step(State* state, State* derivative, double dt);
@@ -33,7 +35,7 @@ void one_step(State* state, State* derivative, double dt);
 // Starting from state, run the simulation until tstop,
 // using dt as time step size.
 // Returns the list of states.
-StateList* run_sim(State state, double tstop, double dt);
+StateList* run_sim(State* state, double tstop, double dt);
 
 extern void * malloc (size_t n);
 extern void exit(int n);
