formal/task01/state_list.c
@@ -1,15 +1,31 @@
 #include <stddef.h>
 #include "state.h"
 
-StateList* new_state_list(State data, StateList* next) {
+void copy_state(State* dest, State* src) {
+  int i = 0;
+  while (i < StateSize) {
+    dest->item[i] = src->item[i];
+    i++;
+  }
+}
+
+State* clone_state(State* data) {
+  State* result = (State*)malloc(sizeof(State));
+  if (!result) exit(1);
+  copy_state(result, data);
+  return result;
+}
+
+StateList* new_state_list(State* data, StateList* next) {
+  State* data_copy = clone_state(data);
   StateList* result = (StateList*)malloc(sizeof(StateList));
   if (!result) exit(1);
-  result->data = data;
+  result->data = data_copy;
   result->next = next;
   return result;
 }
 
-StateList* state_list_cons(StateList* list, State item) {
+StateList* state_list_cons(StateList* list, State* item) {
   StateList* cell = new_state_list(item, list);
   return cell;
 }
