formal/task01/list_spec.v
@@ -28,6 +28,46 @@ Definition strchr_spec' {CSX: compspecs} (_strchr _str _c: positive) :=
 
  *)
 
+(*+ Definitions for State structure +*)
+
+(* type of the state cell *)
+Definition tstate := Tstruct _s_state noattr.
+
+(* Type of pointer to state *)
+Definition pstate := tptr tstate.
+
+(* Field ident holding the array of items *)
+Definition item_id := _item.
+
+(* Coq type representing the state *)
+Definition rstate := Eval compute in reptype tstate.
+
+(* Define what it means for a pointer to hold a state cell *)
+Definition state_cell (data: rstate) (p: val): mpred :=
+ data_at Ews tstate data p * malloc_token Ews tstate p.
+
+Definition state_cell_local_facts:
+  forall data p, state_cell data p |-- !! isptr p.
+Proof. intros. unfold state_cell. entailer!. Qed.
+Hint Resolve state_cell_local_facts: saturate_local.
+
+Definition state_cell_valid_pointer:
+  forall data p, state_cell data p |-- valid_pointer p.
+Proof. intros. unfold state_cell. entailer!. Qed.
+Hint Resolve state_cell_valid_pointer: valid_pointer.
+
+Lemma state_cell_fold: forall data p,
+    data_at Ews tstate data p
+    * malloc_token Ews tstate p
+                   |-- state_cell data p.
+Proof.
+  intros.
+  unfold state_cell.
+  entailer!.
+Qed.
+
+(*+ * Definitions for list cells +*)
+
 (* type of the list cell *)
 Definition tcell := Tstruct _s_state_list noattr.
 
@@ -40,6 +80,9 @@ Definition next_id := _next.
 (* Type of the data *)
 Definition tdata := Tstruct _s_state noattr.
 
+(* Type of pointer to data *)
+Definition pdata := tptr tdata.
+
 (* Coq type representing tdata *)
 Definition rdata := Eval compute in reptype tdata.
 
@@ -47,27 +90,42 @@ Definition rdata := Eval compute in reptype tdata.
 Definition rcell := Eval compute in reptype tcell.
 
 (* Define what it means for a pointer to hold a list cell *)
-Definition list_cell (data: rdata) (next: val) (p: val): mpred :=
- data_at Ews tcell (data, next) p * malloc_token Ews tcell p.
+Definition list_cell (data: rstate) (next: val) (p: val): mpred :=
+  EX datap: val,
+            data_at Ews tcell (datap, next) p *
+            malloc_token Ews tcell p *
+            state_cell data datap.
 
 Definition list_cell_local_facts:
   forall data next p, list_cell data next p |-- !! isptr p.
-Proof. intros. unfold list_cell. entailer!. Qed.
+Proof.
+  intros.
+  unfold list_cell.
+  entailer.
+  unfold state_cell.
+  entailer.
+Qed.
 Hint Resolve list_cell_local_facts: saturate_local.
 
 Definition list_cell_valid_pointer:
-  forall data next p, list_cell data next p |-- valid_pointer p.
-Proof. intros. unfold list_cell. entailer!. Qed.
+  forall datap next p, list_cell datap next p |-- valid_pointer p.
+Proof.
+  intros.
+  unfold list_cell.
+  entailer.
+Qed.
 Hint Resolve list_cell_valid_pointer: valid_pointer.
 
-Lemma listcell_fold: forall data p' p,
-    data_at Ews tcell (data, p') p
-    * malloc_token Ews tcell p
+Lemma listcell_fold: forall data datap p' p,
+    data_at Ews tcell (datap, p') p *
+    malloc_token Ews tcell p *
+    state_cell data datap
                    |-- list_cell data p' p.
 Proof.
   intros.
   unfold list_cell.
-  entailer!.
+  Exists datap.
+  entailer.
 Qed.
 
 Fixpoint listrep (sigma: list rdata) (x: val) : mpred :=
@@ -125,13 +183,162 @@ Qed.
 
 Hint Resolve listrep_valid_pointer : valid_pointer.
 
+Definition copy_state_id := _copy_state.
+Definition copy_state_arg0_id := _dest.
+Definition copy_state_arg1_id := _src.
+
+Definition copy_state_spec : ident * funspec :=
+ DECLARE copy_state_id
+ WITH shsrc: share, shdest: share, 
+      datasrc: rdata, deaddata: rdata, 
+      srcp: val, destp: val, gv: globals
+ PRE [ copy_state_arg0_id OF pstate,
+       copy_state_arg1_id OF pstate ]
+   PROP(readable_share shsrc; writable_share shdest)
+   LOCAL(temp copy_state_arg0_id destp;
+           temp copy_state_arg1_id srcp;
+           gvars gv)
+   SEP(mem_mgr gv;
+         state_cell datasrc srcp;
+         state_cell deaddata destp
+      )
+ POST [ tvoid ]
+      PROP()
+      LOCAL()
+      SEP(state_cell datasrc srcp; state_cell datasrc destp; mem_mgr gv).
+
+Definition Gprog : funspecs :=
+        ltac:(with_library prog [
+                   copy_state_spec 
+ ]).
+
+Lemma body_copy_state: semax_body Vprog Gprog f_copy_state copy_state_spec.
+Proof.
+  start_function.
+  forward.
+  forward_while
+    (exp (fun i:Z =>
+        (PROP(0 <= i <= 3)
+         LOCAL(temp _i (Vint (Int.repr i));
+               temp copy_state_arg0_id destp;
+               temp copy_state_arg1_id srcp;
+               gvars gv)
+         SEP(mem_mgr gv;
+             state_cell datasrc srcp;
+             state_cell
+               ((sublist 0 i datasrc) ++ (sublist i 3 deaddata))
+               destp)
+        ))).
+
+  forward_while
+  
+  forward_for_simple_bound 3
+     (EX: i,
+        PROP()
+        LOCAL(temp copy_state_arg0_id destp; temp copy_state_arg1_id srcp; 
+              gvars gv)
+        SEP(mem_mgr gv; state_cell datasrc srcp; 
+            state_cell deaddata destp)
+     ).
+  exp
+  check_Delta.
+  check_POSTCONDITION.
+ repeat match goal with |-
+      semax _ _ (Ssequence (Ssequence (Ssequence _ _) _) _) _ =>
+      apply -> seq_assoc; abbreviate_semax
+ end.
+ match goal with |-
+      semax _ _ (Ssequence (Ssequence (Sfor _ _ _ _) _) _) _ =>
+      apply -> seq_assoc; abbreviate_semax
+ | _ => idtac
+ end.
+ Check PROP()
+        LOCAL(temp copy_state_arg0_id destp; temp copy_state_arg1_id srcp; 
+              gvars gv)
+        SEP(mem_mgr gv; state_cell datasrc srcp; 
+            state_cell deaddata destp)%assert.
+ 
+ first [
+    match type of n with
+      ?t => first [ unify t Z | elimtype (Type_of_bound_in_forward_for_should_be_Z_but_is t)]
+    end;
+    match type of Pre with
+      ?t => first [unify t (environ -> mpred); fail 1 | elimtype (Type_of_invariant_in_forward_for_should_be_environ_arrow_mpred_but_is t)]
+    end
+  | match goal with
+    | |- semax _ _ (Sfor _ _ _ _) _ =>
+           rewrite semax_seq_skip
+    | |- semax _ _ (Ssequence _ (Sloop _ _)) _ =>
+           rewrite semax_seq_skip
+    | |- semax _ _ (Ssequence _ ?MORE_COMMANDS) _ =>
+        revert MORE_COMMANDS;
+        match goal with
+        | |- let MORE_COMMANDS := @abbreviate _ (Sloop _ _) in _ =>
+            intros MORE_COMMANDS;
+            rewrite semax_seq_skip
+        end
+    | _ => idtac
+    end;
+    forward_for_simple_bound'' n Pre; [.. | abbreviate_semax; cbv beta; try fwd_skip]
+  ].
+  forward_for_simple_bound 3
+     (EX: i,
+        PROP()
+        LOCAL(temp copy_state_arg0_id destp; temp copy_state_arg1_id srcp; 
+              gvars gv)
+        SEP(mem_mgr gv; state_cell datasrc srcp; 
+            state_cell deaddata destp)
+     )%assert.
+  
+Qed.
+
+Definition clone_state_id := _clone_state.
+Definition clone_state_arg0_id := _data.
+
+Definition clone_state_spec : ident * funspec :=
+ DECLARE clone_state_id
+ WITH sh: share, data: rdata, datap: val, gv: globals
+ PRE [ clone_state_arg0_id OF pstate ]
+   PROP(readable_share sh)
+   LOCAL(temp clone_state_arg0_id datap; gvars gv)
+   SEP(mem_mgr gv; state_cell data datap)
+ POST [ pstate ]
+   EX p:val, PROP()
+      LOCAL(temp ret_temp p)
+      SEP(state_cell data datap; state_cell data p; mem_mgr gv).
+
+
+(*+  Putting all the funspecs together +*)
+
+Definition Gprog : funspecs :=
+        ltac:(with_library prog [
+                   copy_state_spec clone_state_spec
+ ]).
+
+
+(*+ Body Proofs +*)
+
+Lemma body_copy_state: semax_body Vprog Gprog f_copy_state copy_state_spec.
+Proof.
+  start_function.
+Qed.
+
+
+
+Lemma body_clone_state: semax_body Vprog Gprog f_clone_state clone_state_spec.
+Proof.
+  start_function.
+Qed.
+
+
+
 Definition new_cell_id := _new_state_list.
 Definition new_cell_spec : ident * funspec :=
  DECLARE new_cell_id
- WITH sh: share, data: rdata, next: val, gv: globals
- PRE [ data_id OF rdata, next_id OF tptr tcell ]
+ WITH sh: share, data: rdata, datap: val, next: val, gv: globals
+ PRE [ data_id OF tdata, next_id OF tptr tcell ]
    PROP(readable_share sh)
-   LOCAL(temp data_id data; temp next_id next; gvars gv)
+   LOCAL(temp data_id val; temp next_id next; gvars gv)
    SEP(mem_mgr gv)
  POST [ tptr tcell ]
    EX p:val, PROP()
