formal/coqimp/digsim5.v
@@ -1,0 +1,273 @@
+(** DigSim
+
+   DigSim provides a Coq architecture required to simulate continuous systems
+   described by sets of simultaneous first-order differential equations.
+
+     xdd := -(spring_coefficient*x + damping_coefficient*xd)/mass - gravity;
+
+
+ ** _CoqProject config file contents
+
+   -R ~/opt/lib/compcert/coq compcert -R . Top
+
+ *)
+
+Require Import DigUty.float_text_io.
+Require Import DigUty.Monad.
+
+From compcert Require Import Floats.
+Import Float.
+From compcert Require Import Fappli_IEEE.
+From compcert Require Import Integers.
+Require Import Coq.Lists.List.
+Import ListNotations.
+Require Import BinNums.
+Require Import Coq.QArith.QArith_base.
+Require Import Strings.String.
+Require Import Strings.Ascii.
+Require Import Coq.ZArith.Znat.
+Require Import Recdef.
+From compcert Require Import Maps.
+Import FloatIO.
+From RecordUpdate Require Import RecordUpdate.
+
+(* Inductive type used to name state variables. *)
+Inductive StateVar : Set := 
+| svT
+| svX
+| svXD
+| svXDD
+| svCOEFF_OF_REST
+| svGRAVITY
+| svT_STOP
+| svDT
+| svDT_MAX
+| svDT_MIN
+| svDT_PRINT.
+
+Lemma state_var_eq: forall (r1 r2: StateVar), {r1 = r2} + {r1 <> r2}.
+Proof. decide equality. Defined.
+Global Opaque state_var_eq.
+
+From compcert Require Import Decidableplus.
+
+Instance Decidable_eq_sv : forall (x y: StateVar), Decidable (eq x y) := Decidable_eq state_var_eq.
+
+(* For diagnostic purposes we want to map from the positive id for a
+   StateVar to the StateVar. 
+ *)
+Definition PosToStateVarTree := PTree.t StateVar.
+Definition EmptyPosToStateVarTree := PTree.empty StateVar.
+
+Definition SvIndex (sv: StateVar) : positive :=
+  match sv with
+  | svT => 1
+  | svX => 2
+  | svXD => 3
+  | svXDD => 4
+  | svCOEFF_OF_REST => 5
+  | svGRAVITY => 6
+  | svT_STOP => 7
+  | svDT => 8
+  | svDT_MAX => 9
+  | svDT_MIN => 10
+  | svDT_PRINT => 11
+  end.
+
+Definition SvStrList :=
+  [
+    (svT, "T");
+    (svX, "X");
+    (svXD, "XD");
+    (svXDD, "XDD");
+    (svCOEFF_OF_REST, "COEFF_OF_REST");
+    (svGRAVITY, "GRAVITY");
+    (svT_STOP, "T_STOP");
+    (svDT, "DT");
+    (svDT_MAX, "DT_MAX");
+    (svDT_MIN, "DT_MIN");
+    (svDT_PRINT, "DT_PRINT")
+  ]%positive.
+
+Fixpoint UpdatePosToStateVarTree (svIdStrList: list (StateVar * string))
+         (tree: PosToStateVarTree) : PosToStateVarTree :=
+  match svIdStrList with
+  | nil => tree
+  | cons (sv, str) xtail =>
+    let tree1 := PTree.set (SvIndex sv) sv tree in
+    UpdatePosToStateVarTree xtail tree1
+  end.
+
+Definition posToStateVarTree :=
+  Eval compute in UpdatePosToStateVarTree SvStrList EmptyPosToStateVarTree.
+
+Definition posToStateVar (p: positive) := PTree.get p posToStateVarTree.
+
+(*
+Compute PTree.elements posToStateVarTree.
+Compute posToStateVar 3.
+*)
+
+Module SvIndex <: Maps.INDEXED_TYPE.
+  Definition t := StateVar.
+  Definition index := SvIndex.
+  Definition eq := state_var_eq.
+  Lemma index_inj:
+    forall r1 r2, index r1 = index r2 -> r1 = r2.
+  Proof.
+    intros.
+    destruct r1 eqn: r1eq; destruct r2 eqn: r2eq; simpl in *;try reflexivity;
+      unfold index in H; simpl in H; inversion H.
+  Qed.
+End SvIndex.
+
+Module SvTree := Maps.ITree(SvIndex).
+
+Definition StringSvTree := SvTree.t string.
+Definition emptyStringPTree := SvTree.empty string.
+
+Fixpoint UpdateStringSvTree (valList: list (StateVar * string)) (intree: StringSvTree) :=
+  match valList with
+  | nil => intree
+  | cons (sv, val) vltail =>
+    let tree1 := SvTree.set sv val intree in
+    UpdateStringSvTree vltail tree1
+  end.
+
+Definition svToStringTree :=
+  Eval compute in UpdateStringSvTree SvStrList emptyStringPTree.
+
+Definition svToStrOpt (sv: StateVar) : option string :=
+  SvTree.get sv svToStringTree.
+
+Lemma svToStrComplete:
+  forall sv : StateVar, exists s : string,
+      svToStrOpt sv = Some s.
+Proof.
+  intros.
+  destruct sv; unfold svToStrOpt;compute; eexists; f_equal.
+Qed.
+
+(* Since we have proven that svToStrOpt will always give a 
+   result, define a function that extracts that value,
+   and in the impossible case returns the empty string.
+*)
+Definition svToStr (sv: StateVar) : string :=
+  match svToStrOpt sv with
+  | Some x => x
+  | None => ""
+  end.
+
+(*
+Compute svToStr svDT.
+Compute svToStr svDT_PRINT.
+*)
+
+Definition FloatSvTree := SvTree.t float.
+Definition emptyFloatPTree := SvTree.empty float.
+
+Fixpoint UpdateFloatSvTree (valList: list (StateVar * string)) (intree: FloatSvTree) :=
+  match valList with
+  | nil => intree
+  | cons (sv, str) vltail =>
+    let tree1 :=
+    match strToFloat str with
+    | Some val => SvTree.set sv val intree
+    | None => intree
+    end in
+    UpdateFloatSvTree vltail tree1
+  end.
+
+Definition initialValues :=
+  [
+    (svT,             "0.0");
+    (svX,             "10.0");
+    (svXD,            "0.0");
+    (svXDD,           "0.0");
+    (svCOEFF_OF_REST, "0.80");
+    (svGRAVITY,       "9.88");
+    (svT_STOP,        "10.0");
+    (svDT,            "0.01");
+    (svDT_MAX,        "0.005");
+    (svDT_MIN,        "0.001");
+    (svDT_PRINT,      "0.01")
+  ].
+
+Definition state0 := Eval compute in UpdateFloatSvTree initialValues emptyFloatPTree.
+
+Definition svToFloat0 (sv: StateVar) := SvTree.get sv state0.
+
+Definition svToFloatStr0 (sv: StateVar) :=
+  match svToFloat0 sv with
+  | Some x => float_to_string 8 4 x
+  | None => "None"
+  end.
+
+Compute svToFloatStr0 svGRAVITY.
+
+Lemma state0Complete:
+  forall sv: StateVar, exists f: float,
+      SvTree.get sv state0 = Some f.
+Proof.
+  intros.
+  destruct sv;compute; eexists; f_equal.
+Qed.
+
+(*
+Compute SvTree.get svXD (SvTree.set svXD Float.zero emptyFloatPTree).
+*)
+
+Definition modelOutputs : list StateVar := [svT; svX; svXD].
+Print modelOutputs.
+
+
+
+Definition ident := term.
+    
+
+Definition _time: ident := 1.
+
+
+(** DigSim - Mass Spring Damper
+ *)
+Definition time0               := Z_to_float 0                    . (* 0.0          simulation time [sec]                      *)
+Definition x_ic                := Z_to_float 0                    . (* 0.0          initial position of suspended mass [m]     *)
+Definition xd_ic               := Z_to_float 0                    . (* 0.0          initial velocity of suspended mass [m/sec] *)
+Definition mass                := Z_to_float 1                    . (* 1.0    1#1   mass suspended from spring [kg]            *)
+Definition tstop               := fraction_to_float  25  1        . (* 2.5    2#5   simulation stop time [sec]                 *)
+Definition dt                  := fraction_to_float   1  2        . (* 0.01   1#100 simulation time step [sec]                 *)
+Definition damping_coefficient := fraction_to_float 888  2        . (* 8.88 222#25  damping force per velocity [n/m/s]         *)
+Definition gravity             := fraction_to_float 988  2        . (* 9.88 247#25  acceleration due to gravity [m/sec**2]     *)
+Definition spring_coefficient  := fraction_to_float 3947 2        . (* 39.47 3947#100 restoring force per position [n/m]       *)
+
+Open Scope Z.
+
+Definition xdd x xd : float :=
+  sub ( div (neg (add (mul spring_coefficient x)  (mul damping_coefficient xd)) ) mass) gravity.
+
+Definition step (t x xd : float) : (float * float * float) :=
+  let xdd' := xdd x xd             in
+  let x'   := add x  (mul xd   dt) in
+  let xd'  := add xd (mul xdd' dt) in
+  let t'   := add t dt             in
+  (t', x', xd').
+
+Fixpoint advance (fuel : nat) (t x xd : float) : list (list float) :=
+match fuel with
+|  O   => nil
+|  S n =>
+   let '(t', x', xd') := (step t x xd) in
+   (t' :: x' :: xd' :: nil) :: (advance n t' x' xd')
+end.
+
+Definition width := 15%nat.
+Definition fdigs := 6%nat.
+Definition f2s := float_to_string width fdigs.
+Definition fl2s := float_list_to_string width fdigs true.
+
+Definition digsim : string := nl ++ (fl2s (time0 :: x_ic :: xd_ic :: nil)) ++
+                        (concat "" (map fl2s (advance 250 time0 x_ic xd_ic))) ++ nl.
+
+Set Printing Depth 500.
+Set Printing Width 0.
+Compute digsim.
