formal/pi/verif_pi.v
@@ -1,0 +1,32 @@
+(* Verify simple double floating add. *)
+Require Import VST.floyd.proofauto.
+Require Import Pi.pi.
+(* The next line is "boilerplate", always required after importing an AST. *)
+Instance CompSpecs : compspecs. make_compspecs prog. Defined.
+Definition Vprog : varspecs.  mk_varspecs prog. Defined.
+
+Definition pi_spec :=
+  DECLARE _pi
+    WITH z : Z
+    PRE [ ]
+    PROP( )
+    LOCAL()
+    SEP ()
+  POST [ tdouble ] 
+    PROP()
+    LOCAL(temp ret_temp (Vfloat (Float.of_bits (Int64.repr 4614256656552045848))))
+    SEP ().
+
+Definition Gprog : funspecs :=
+    ltac:(with_library prog [
+    pi_spec
+  ]).
+
+Lemma body_pi: semax_body Vprog Gprog f_pi pi_spec.
+Proof.
+  start_function.
+  forward.
+  forward.
+Qed.
+
+
